%chapter 4, Tom Mulvey, 3/7/18
\documentclass[12pt]{article}

\usepackage{amsfonts}
\usepackage{amsmath}
\usepackage{amssymb}
\usepackage{amsthm}
\usepackage{xcolor}
\usepackage{graphicx}
\usepackage{microtype}

%new macros for r,q,n,z
\newcommand{\Q}{\mathbb Q}
\newcommand{\N}{\mathbb N}
\newcommand{\Z}{\mathbb Z}
\newcommand{\R}{\mathbb R}
\newcommand{\ind}{\hspace{10mm}}

\newtheorem{thm}{Theorem}
\newtheorem{lem}[thm]{Lemma}
\newtheorem{cor}[thm]{Corollary}
\newtheorem{rem}[thm]{Remark}
\newtheorem{conj}[thm]{Conjecture}

%\fboxsep=2mm \fboxrule=1mm \fcolorbox{black}{blue!20!white}{\null}
%\fbox{\includegraphics[height=1cm]{proof.png}}
%{%
%	\setlength{\fboxsep}{1pt}%
%	\setlength{\fboxrule}{2pt}%
%	\fbox{\includegraphics[height=1cm]{proof.png}}
%}%

\begin{document}
    \centerline{\sc \large Tom Mulvey | Homework 6 }
    \centerline{\sc 4/5/18}

    \vspace{2pc}

	\begin{enumerate}
		\item[6.8]) Find a formula for $ 1 + 4 + 7 + ... + (3n - 2) $ for positive integers $n$ and then verify
		your formula by mathematical induction.
		
		$Proof : $
		
		\ind Notice that $ 1 + 4 + 7 + ... + (3n - 2) = \frac{n(3n - 1)}{2}$.
		
		\ind We employ induction. Since $1 = \frac{1(3(1) - 1)}{2} = \frac{(3-1)}{2} = \frac{2}{2} $, the
		
		\ind initial statement holds when n=1. Assume that 
		
		\ind \ind $ 1 + 4 + 7 + ... + (3k - 2) = \frac{k(3k - 1)}{2}$ where $k \in \Z +$
		
		\ind We show that
		
		\ind \ind $ 1 + 4 + 7 + ... + (3k - 2) + (3(k+1)-2) = \frac{(k+1)(3(k+1)-2)}{2}$.
		
		\ind Thus $ 1 + 4 + 7 + ... + (3k - 2) + (3(k+1)-2) = \frac{k(3k - 1)}{2} + (3(k+1)-2) $.
		
		\ind $\iff$ $ \frac{k(3k - 1)}{2} + (3(k+1)-2) = \frac{k(3k - 1)}{2} + (3k + 1) $.
		
		\ind $\iff$ $ \frac{k(3k - 1)}{2} + (3k + 1) = \frac{k(3k - 1)}{2} + \frac{2(3k + 1)}{2}  $.		
		
		\ind $\iff$ $ \frac{k(3k - 1)}{2} + \frac{2(3k + 1)}{2} = \frac{k(3k-1) + 2(3k+1)}{2}  $.
		
		\ind $\iff$ $ \frac{k(3k-1) + 2(3k+1)}{2} = \frac{3k^2 - k + 6k + 2}{2} $.
		
		\ind $\iff$ $ \frac{3k^2 - 1k + 6k + 2}{2} = \frac{3k^2 + 5k + 2}{2}  $.
		
		\ind $\iff$ $ \frac{3k^2 - 1k + 6k + 2}{2} = \frac{(k+1)(3k+2)}{2}  $.
		
		\ind $\iff$ $ \frac{3k^2 - 1k + 6k + 2}{2} = \frac{(k+1)(3(k+1)-1)}{2}  $.
		
		\ind \ind By the principle of mathematical induction, $ 1 + 4 + 7 + ... + (3n - 2) = \frac{n(3n - 1)}{2}
		\forall n \in \Z + $				

		\ind \ind \ind \ind \ind \ind 
		{%
			\setlength{\fboxsep}{1pt}%
			\setlength{\fboxrule}{2pt}%
			\fbox{\includegraphics[height=1cm]{proof.png}}
		}%
		
			
		\item[6.22]) Prove that $3^n$ $>$ $n^2$ $\forall n $ s.t. $ n \in \Z +$
		
		$Proof : $
		
		\ind Observe that $3^1$ $>$ $(1)^2$ $\Rightarrow$ $3 > 1$, thus the statement holds when $n=1$.
		
		\ind We will prove this statement using mathematical induction. 
		 
		\ind \ind Assume that $3^k$ $>$ $k^2$ where $k \in \Z +$.
		
		\ind We show that $3^{(k+1)}$ $>$ $(k+1)^2$.
		
		\ind $\iff$ $ 3*3^k$ $>$ $(k+1)^2 = k^2 + 2k + 1 $.
		
		\ind $\iff$ $ 3*3^k$ $>$ $ 2k^2 $  $>$ $ k^2 + 2k + 1 $ (when $ k \geq 3$ ).

		\ind \ind Since the inequality will only hold when $ k \geq 3$, I will show
		
		\ind \ind two more base cases besides n = 1.

		\ind \ind n = 2 $\Rightarrow$ $3^2 > 2^2$ $\Rightarrow$ $ 9 > 4 $.		

		\ind \ind n = 3 $\Rightarrow$ $3^3 > 2^3$ $\Rightarrow$ $ 27 > 9 $.
		
		Since n = 1, 2, and all n $\geq$ 3 all hold true, then by mathematical induction $3^n$ $>$ $n^2$ 
		$\forall n $ s.t. $ n \in \Z +$. 

		\ind \ind \ind \ind \ind \ind 
		{%
			\setlength{\fboxsep}{1pt}%
			\setlength{\fboxrule}{2pt}%
			\fbox{\includegraphics[height=1cm]{proof.png}}
		}%
		
		\item[6.26]) Prove that $ 81 | (10^{n+1} -9n -10)$ $\forall$ $n \in \N $.
		
		$Proof : $
		
		\ind We will employ weak induction. See that when
		
		\ind $n=0$, $ 81 | (10^{0+1} -9(0) -10)$. $\Rightarrow$ $n=0$, $ 81 | 10 - 10)$ $\Rightarrow$ $ 81 | 0$.
		
		\ind This is obvious because 81 * 0 = 0.
		
		\ind $ 81 | (10^{n+1} -9n -10)$ $\Rightarrow$ $\exists$ $x$ $s.t$ $81x = (10^{n+1} -9n -10)$.
		
		\ind Solving for $ 10^{n+1} $ yields $ 81x + 9n + 10$ $=$ $10^{n+1}$.
		
		\ind We must show that $ 81 | (10^{k+1+1} -9(k+1) -10)$, where $k \in \N$.
				
		\ind \ind $(10^{k+1+1} -9(k+1) -10)$ $\iff$ $(10*10^{k+1} -9k -9 -10)$. 
		
		\ind \ind $(10*10^{k+1} -9n -9 -10)$ $\iff$ $(10*(81x + 9k + 10) -9n -19)$.
		
		\ind \ind (recall solving for $10^{k+1}$ )
		
		\ind \ind $(10*(81x + 9k + 10) -9k -19)$ $\iff$ $810x + 90k + 100 -9k -19$.		
		
		\ind \ind $810x + 90k + 100 -9n -19$ $\iff$ $810x + 81k + 81$.		
		
		\ind \ind $810x + 81k + 81$ $\iff$ $81(10x + k + 1)$, 
		
		\ind \ind and since $(10x + k + 1)$ $\in \Z$, 81 divides $(10x + k + 1)$.
		
		\ind By the mathematical induction $ 81 | (10^{n+1} -9n -10)$ $\forall n $ s.t. $ n \in \N$. 
		
		\ind \ind \ind \ind \ind \ind 
		{%
			\setlength{\fboxsep}{1pt}%
			\setlength{\fboxrule}{2pt}%
			\fbox{\includegraphics[height=1cm]{proof.png}}
		}%		
		
		\item[6.34]) A sequence $\{a_n\}$ is defined recursively by $a_1$ $=1$ and $a_2$ $=2$ and $a_n = a_{n-1}
		+ 2*a_{n-}$ $\forall n \geq 3$. Conjecture a formula for $a_n$ and validate it.
		
		$a_n$ = $2^{k-1}$.		
		
		$Proof : $
		
		\ind We will utilize strong induction! I First observe that
		
		\ind \ind $a_1$ = $2^0$ = $1$, and $a_2$ = $2^1$ = $2$. 
		
		\ind This shows that $a_n$ holds when n=1 and n=2.
		
		\ind Assume the formula holds from 1 to $k$ where $ k \geq 1$. 
		
		\ind $a_i$ = $2^{i-1}$   $\forall$ $i\in\Z$ where 1$\leq$i$\leq$k.
		
		\ind We will prove that $a_{k+1}$ = $2^{(k+1)-1}$ = $2^k$.
		
		\ind Notice each recursion call traces back two steps, so 
		
		\ind \ind we will solve when $k \geq 3$. This is fine
		
		\ind \ind since k=1 and k=2 are base cases.
		
		\ind Now $a_{k+1}$ = $2^{k-1}$ + $2*2^{k-2}$.
		
		\ind $\iff$ $a_{k+1}$ = $2^{k-1}$ + $2^{k-2+1}$ = $2*2^{k-1}$ = $2^k$.
		
		\ind By the mathematical induction . 
		
		\ind \ind \ind \ind \ind \ind 
		{%
			\setlength{\fboxsep}{1pt}%
			\setlength{\fboxrule}{2pt}%
			\fbox{\includegraphics[height=1cm]{proof.png}}
		}%		
			 		
	\end{enumerate}

\end {document}